ProvabilityLogic/Logic/Basic.lean
@@ -1,6 +1,6 @@
 module
 
-public import ProvabilityLogic.Hilbert.Basic
+public import ProvabilityLogic.Hilbert.GL.Basic
 public import ProvabilityLogic.Kripke.Cone
 
 @[expose]
